driver/Compiler.v
@@ -52,7 +52,7 @@ Require Inlining.
 Require Renumber.
 Require Constprop.
 Require CSE.
-(*Require Deadcode.*)
+Require Deadcode.
 (*Require Unusedglob.*)
 Require Allocation.
 Require Tunneling.
@@ -73,7 +73,7 @@ Require Inliningproof.
 Require Renumberproof.
 Require Constpropproof.
 Require CSEproof.
-(*Require Deadcodeproof.*)
+Require Deadcodeproof.
 (*Require Unusedglobproof.*)
 Require Allocproof.
 Require Tunnelingproof.
@@ -144,9 +144,9 @@ Definition transf_rtl_program (f: RTL.program) : res Asm.program :=
   !@@ print (print_RTL 5)
   @@@ partial_if Compopts.optim_CSE (time "CSE" CSE.transf_program)
   !@@ print (print_RTL 6)
-(*
   @@@ partial_if Compopts.optim_redundancy (time "Redundancy elimination" Deadcode.transf_program)
-   @@ print (print_RTL 7)
+  !@@ print (print_RTL 7)
+(*
   @@@ time "Unused globals" Unusedglob.transform_program
    @@ print (print_RTL 8)
 *)
@@ -260,8 +260,8 @@ Definition CompCert's_passes :=
   ::: mkpass (match_if Compopts.optim_constprop Constpropproof.match_prog)
   ::: mkpass (match_if Compopts.optim_constprop Renumberproof.match_prog)
   ::: mkpass (match_if Compopts.optim_CSE CSEproof.match_prog)
-(*
   ::: mkpass (match_if Compopts.optim_redundancy Deadcodeproof.match_prog)
+(*
   ::: mkpass Unusedglobproof.match_prog
 *)
   ::: mkpass Allocproof.match_prog
@@ -313,11 +313,11 @@ Proof.
   set (p10 := total_if optim_constprop Constprop.transf_program p9) in *.
   set (p11 := total_if optim_constprop Renumber.transf_program p10) in *.
   destruct (partial_if optim_CSE CSE.transf_program p11) as [p12|e] eqn:P12; simpl in T; try discriminate.
-  (*
   destruct (partial_if optim_redundancy Deadcode.transf_program p12) as [p13|e] eqn:P13; simpl in T; try discriminate.
+  (*
   destruct (Unusedglob.transform_program p13) as [p14|e] eqn:P14; simpl in T; try discriminate.
    *)
-  destruct (Allocation.transf_program p12) as [p15|e] eqn:P15; simpl in T; try discriminate.
+  destruct (Allocation.transf_program p13) as [p15|e] eqn:P15; simpl in T; try discriminate.
   set (p16 := Tunneling.tunnel_program p15) in *.
   destruct (Linearize.transf_program p16) as [p17|e] eqn:P17; simpl in T; try discriminate.
   set (p18 := CleanupLabels.transf_program p17) in *.
@@ -338,8 +338,8 @@ Proof.
   exists p10; split. apply total_if_match. apply Constpropproof.transf_program_match.
   exists p11; split. apply total_if_match. apply Renumberproof.transf_program_match.
   exists p12; split. eapply partial_if_match; eauto. apply CSEproof.transf_program_match.
-  (*
   exists p13; split. eapply partial_if_match; eauto. apply Deadcodeproof.transf_program_match.
+  (*
   exists p14; split. apply Unusedglobproof.transf_program_match; auto.
    *)
   exists p15; split. apply Allocproof.transf_program_match; auto.
@@ -417,6 +417,7 @@ Qed.
 Definition cc_backend : callconv li_c Asm.li_asm :=
   cc_inj @
   ((Invariant.cc_inv ValueAnalysis.vamatch @ cc_ext) @ cc_id) @
+  (Invariant.cc_inv ValueAnalysis.vamatch @ cc_ext) @
   (Invariant.cc_inv ValueAnalysis.vamatch @ cc_ext) @
   Conventions.cc_alloc @
   Conventions.cc_locset_ext @
@@ -553,7 +554,7 @@ Ltac DestructM :=
       destruct H as (p & M & MM); clear H
   end.
   repeat DestructM. subst tp.
-  assert (F: forward_simulation cc_compcert cc_compcert (Clight.semantics1 p) (Asm.semantics p18)).
+  assert (F: forward_simulation cc_compcert cc_compcert (Clight.semantics1 p) (Asm.semantics p19)).
   {
   eapply compose_clight_properties.
   (*
@@ -602,9 +603,14 @@ Ltac DestructM :=
       eapply Invariant.preserves_fsim. eapply ValueAnalysis.rtl_vamatch.
       rewrite <- cc_c_ext at 1. rewrite <- cc_c_ext.
       eapply RTLrel.semantics_rel.
-  (*
   eapply compose_forward_simulations.
-    eapply match_if_simulation. eassumption. exact Deadcodeproof.transf_program_correct; eassumption.
+    red in M10. destruct optim_redundancy; subst.
+    eapply Deadcodeproof.transf_program_correct; eauto.
+    eapply compose_forward_simulations.
+      eapply Invariant.preserves_fsim. eapply ValueAnalysis.rtl_vamatch.
+      rewrite <- cc_c_ext at 1. rewrite <- cc_c_ext.
+      eapply RTLrel.semantics_rel.
+  (*
   eapply compose_forward_simulations.
     eapply Unusedglobproof.transf_program_correct; eassumption.
    *)
